proof/iu_system/main.v
@@ -1,0 +1,8 @@
+Require Import ln_utils.
+Require Import uni.def_ott.
+Require Import uni.decl.def_extra.
+Require Import uni.notations.
+Require Import uni.prop_basic.
+Require Import uni.decl_worklist.prop_equiv.
+Require Import uni.algo_worklist.transfer.
+Require Import uni.algo_worklist.def_extra.
