proof/iu_system/prop_safety.v
@@ -3,9 +3,8 @@ Require Import uni.def_ott.
 Require Import uni.decl.def_extra.
 Require Import uni.notations.
 Require Import uni.prop_basic.
-Require Import uni.decl_worklist.prop_equiv.
-Require Import uni.decl.prop_subtyping.
 Require Import uni.prop_basic.
+Require Import uni.decl.prop_subtyping.
 
 
 Require Import systemf.def_ott.
