proof/iu_system/uni/algo_worklist/prop_soundness.v
@@ -1,0 +1,35 @@
+Require Import Coq.Program.Equality.
+Require Import Program.Tactics.
+Require Import Metalib.Metatheory.
+Require Import List.
+
+
+Require Import uni.notations.
+Require Import uni.algo_worklist.def_extra.
+Require Import uni.algo_worklist.transfer.
+Require Import ln_utils.
+
+
+Hint Constructors d_wl_del_red : Hdb_a_wl_red_soundness.
+
+
+Theorem d_a_wl_red_soundness: forall Γ,
+  ⊢ᵃ Γ -> Γ ⟶ᵃʷ⁎⋅ -> exists Ω, transfer Γ Ω /\ Ω ⟶ᵈ⁎⋅.
+Proof with auto with Hdb_a_wl_red_soundness.
+  intros. induction H0; auto; unfold transfer in *.
+  - dependent destruction H.
+    apply IHa_wl_red in H1.
+    destruct H1 as [Ω [Htr Hd_red]].
+    admit.
+  - dependent destruction H. 
+    apply IHa_wl_red in H0.
+    destruct H0 as [Ω [Htrans Hd_red]].
+    destruct Htrans as [θ Htrans].
+    exists (dworklist_constvar Ω X dbind_tvar_empty).
+    econstructor. exists ((X, ss_bind__tvar_empty) :: θ).
+    apply inst_wl__cons_tvar; auto.
+    econstructor...
+  - admit.
+  - admit.
+  -
+Admitted.
